Interfaces; hints

ulib/FStar.Endianness.fst
@@ -23,32 +23,21 @@ module U64 = FStar.UInt64
 module Math = FStar.Math.Lemmas
 module S = FStar.Seq
 
-noextract
-type bytes = S.seq U8.t
-
 open FStar.Mul
 
 /// Definition of little and big-endianness
 /// ---------------------------------------
-///
-/// This is our spec, to be audited. From bytes to nat.
 
-/// lt_to_n interprets a byte sequence as a little-endian natural number
-val le_to_n : b:bytes -> Tot nat (decreases (S.length b))
 let rec le_to_n b =
   if S.length b = 0 then 0
   else U8.v (S.head b) + pow2 8 * le_to_n (S.tail b)
 
-/// be_to_n interprets a byte sequence as a big-endian natural number
-val be_to_n : b:bytes -> Tot nat (decreases (S.length b))
-let rec be_to_n b =
+let rec be_to_n b: Tot nat (decreases (S.length b)) =
   if S.length b = 0 then 0
   else U8.v (S.last b) + pow2 8 * be_to_n (S.slice b 0 (S.length b - 1))
 
 /// Inverse operations
 /// ------------------
-///
-/// From nat to bytes, and their functional correctness.
 
 /// TODO: move to FStar.Math.Lemmas?
 private val lemma_euclidean_division: r:nat -> b:nat -> q:pos -> Lemma
@@ -60,10 +49,6 @@ let lemma_euclidean_division r b q = ()
 private val lemma_factorise: a:nat -> b:nat -> Lemma (a + a * b == a * (b + 1))
 let lemma_factorise a b = ()
 
-val lemma_le_to_n_is_bounded: b:bytes -> Lemma
-  (requires True)
-  (ensures  (le_to_n b < pow2 (8 * Seq.length b)))
-  (decreases (Seq.length b))
 let rec lemma_le_to_n_is_bounded b =
   if Seq.length b = 0 then ()
   else
@@ -81,10 +66,6 @@ let rec lemma_le_to_n_is_bounded b =
     lemma_factorise 8 (Seq.length b - 1)
     end
 
-val lemma_be_to_n_is_bounded: b:bytes -> Lemma
-  (requires True)
-  (ensures  (be_to_n b < pow2 (8 * Seq.length b)))
-  (decreases (Seq.length b))
 let rec lemma_be_to_n_is_bounded b =
   if Seq.length b = 0 then ()
   else
@@ -102,11 +83,6 @@ let rec lemma_be_to_n_is_bounded b =
     lemma_factorise 8 (Seq.length b - 1)
     end
 
-/// n_to_le encodes a number as a little-endian byte sequence of a fixed,
-/// sufficiently large length.
-val n_to_le : len:nat -> n:nat{n < pow2 (8 * len)} ->
-  Tot (b:bytes{S.length b == len /\ n == le_to_n b})
-  (decreases len)
 let rec n_to_le len n =
   if len = 0 then
     S.empty
@@ -121,12 +97,6 @@ let rec n_to_le len n =
     S.lemma_eq_intro b' (S.tail b);
     b
 
-/// n_to_be encodes a numbers as a big-endian byte sequence of a fixed,
-/// sufficiently large length
-val n_to_be:
-  len:nat -> n:nat{n < pow2 (8 * len)} ->
-  Tot (b:bytes{S.length b == len /\ n == be_to_n b})
-  (decreases len)
 let rec n_to_be len n =
   if len = 0 then
     S.empty
@@ -144,25 +114,14 @@ let rec n_to_be len n =
 /// Injectivity
 /// -----------
 
-let n_to_le_inj (len: nat) (n1 n2: (n:nat{n < pow2 (8 * len)})) :
-  Lemma (requires (n_to_le len n1 == n_to_le len n2))
-        (ensures (n1 == n2)) =
-  // this lemma easily follows from le_to_n . (n_to_le len) == id, the inversion
-  // proof in the spec for n_to_le
-  ()
+// this lemma easily follows from le_to_n . (n_to_le len) == id, the inversion
+// proof in the spec for n_to_le
+let n_to_le_inj len n1 n2 = ()
 
-let n_to_be_inj (len: nat) (n1 n2: (n:nat{n < pow2 (8 * len)})) :
-  Lemma (requires (n_to_be len n1 == n_to_be len n2))
-        (ensures (n1 == n2)) =
-  ()
+let n_to_be_inj len n1 n2 = ()
 
-let rec be_to_n_inj
-  (b1 b2: Seq.seq U8.t)
-: Lemma
-  (requires (Seq.length b1 == Seq.length b2 /\ be_to_n b1 == be_to_n b2))
-  (ensures (Seq.equal b1 b2))
-  (decreases (Seq.length b1))
-= if Seq.length b1 = 0
+let rec be_to_n_inj b1 b2 =
+  if Seq.length b1 = 0
   then ()
   else begin
     be_to_n_inj (Seq.slice b1 0 (Seq.length b1 - 1)) (Seq.slice b2 0 (Seq.length b2 - 1));
@@ -170,13 +129,8 @@ let rec be_to_n_inj
     Seq.lemma_split b2 (Seq.length b2 - 1)
   end
 
-let rec le_to_n_inj
-  (b1 b2: Seq.seq U8.t)
-: Lemma
-  (requires (Seq.length b1 == Seq.length b2 /\ le_to_n b1 == le_to_n b2))
-  (ensures (Seq.equal b1 b2))
-  (decreases (Seq.length b1))
-= if Seq.length b1 = 0
+let rec le_to_n_inj b1 b2 =
+  if Seq.length b1 = 0
   then ()
   else begin
     le_to_n_inj (Seq.slice b1 1 (Seq.length b1)) (Seq.slice b2 1 (Seq.length b2));
@@ -187,60 +141,14 @@ let rec le_to_n_inj
 /// Roundtripping
 /// -------------
 
-let n_to_be_be_to_n (len: nat) (s: Seq.seq U8.t) : Lemma
-  (requires (Seq.length s == len))
-  (ensures (
-    be_to_n s < pow2 (8 * len) /\
-    n_to_be len (be_to_n s) == s
-  ))
-  [SMTPat (n_to_be len (be_to_n s))]
-= lemma_be_to_n_is_bounded s;
+let n_to_be_be_to_n len s =
+  lemma_be_to_n_is_bounded s;
   be_to_n_inj s (n_to_be len (be_to_n s))
 
-let n_to_le_le_to_n (len: nat) (s: Seq.seq U8.t) : Lemma
-  (requires (Seq.length s == len))
-  (ensures (
-    le_to_n s < pow2 (8 * len) /\
-    n_to_le len (le_to_n s) == s
-  ))
-  [SMTPat (n_to_le len (le_to_n s))]
-= lemma_le_to_n_is_bounded s;
+let n_to_le_le_to_n len s =
+  lemma_le_to_n_is_bounded s;
   le_to_n_inj s (n_to_le len (le_to_n s))
 
-/// Specializations for F* machine integers
-/// ---------------------------------------
-
-let uint32_of_le (b: bytes { S.length b = 4 }) =
-  let n = le_to_n b in
-  lemma_le_to_n_is_bounded b;
-  UInt32.uint_to_t n
-
-let le_of_uint32 (x: UInt32.t): b:bytes{ S.length b = 4 } =
-  n_to_le 4 (UInt32.v x)
-
-let uint32_of_be (b: bytes { S.length b = 4 }) =
-  let n = be_to_n b in
-  lemma_be_to_n_is_bounded b;
-  UInt32.uint_to_t n
-
-let be_of_uint32 (x: UInt32.t): b:bytes{ S.length b = 4 } =
-  n_to_be 4 (UInt32.v x)
-
-let uint64_of_le (b: bytes { S.length b = 8 }) =
-  let n = le_to_n b in
-  lemma_le_to_n_is_bounded b;
-  UInt64.uint_to_t n
-
-let le_of_uint64 (x: UInt64.t): b:bytes{ S.length b = 8 } =
-  n_to_le 8 (UInt64.v x)
-
-let uint64_of_be (b: bytes { S.length b = 8 }) =
-  let n = be_to_n b in
-  lemma_be_to_n_is_bounded b;
-  UInt64.uint_to_t n
-
-let be_of_uint64 (x: UInt64.t): b:bytes{ S.length b = 8 } =
-  n_to_be 8 (UInt64.v x)
 
 /// Reasoning over sequences of integers
 /// ------------------------------------
@@ -249,73 +157,53 @@ let be_of_uint64 (x: UInt64.t): b:bytes{ S.length b = 8 } =
 /// export a variant (which we need for, say, hashes) specialized to F* machine
 /// integers?
 
-let rec seq_uint32_of_le (l: nat) (b: bytes{ S.length b = 4 * l }):
-  s:S.seq UInt32.t { S.length s = l }
-=
+let rec seq_uint32_of_le l b =
   if S.length b = 0 then
     S.empty
   else
     let hd, tl = Seq.split b 4 in
     S.cons (uint32_of_le hd) (seq_uint32_of_le (l - 1) tl)
 
-let rec le_of_seq_uint32 (s: S.seq UInt32.t):
-  Tot (b:bytes { S.length b = 4 * S.length s })
-    (decreases (S.length s))
-=
+let rec le_of_seq_uint32 s =
   if S.length s = 0 then
     S.empty
   else
     S.append (le_of_uint32 (S.head s)) (le_of_seq_uint32 (S.tail s))
 
-let rec seq_uint32_of_be (l: nat) (b: bytes{ S.length b = 4 * l }):
-  s:S.seq UInt32.t { S.length s = l }
-=
+let rec seq_uint32_of_be l b =
   if S.length b = 0 then
     S.empty
   else
     let hd, tl = Seq.split b 4 in
     S.cons (uint32_of_be hd) (seq_uint32_of_be (l - 1) tl)
 
-let rec be_of_seq_uint32 (s: S.seq UInt32.t):
-  Tot (b:bytes { S.length b = 4 * S.length s })
-    (decreases (S.length s))
-=
+let rec be_of_seq_uint32 s =
   if S.length s = 0 then
     S.empty
   else
     S.append (be_of_uint32 (S.head s)) (be_of_seq_uint32 (S.tail s))
 
-let rec seq_uint64_of_le (l: nat) (b: bytes{ S.length b = 8 * l }):
-  s:S.seq UInt64.t { S.length s = l }
-=
+let rec seq_uint64_of_le l b =
   if S.length b = 0 then
     S.empty
   else
     let hd, tl = Seq.split b 8 in
     S.cons (uint64_of_le hd) (seq_uint64_of_le (l - 1) tl)
 
-let rec le_of_seq_uint64 (s: S.seq UInt64.t):
-  Tot (b:bytes { S.length b = 8 * S.length s })
-    (decreases (S.length s))
-=
+let rec le_of_seq_uint64 s =
   if S.length s = 0 then
     S.empty
   else
     S.append (le_of_uint64 (S.head s)) (le_of_seq_uint64 (S.tail s))
 
-let rec seq_uint64_of_be (l: nat) (b: bytes{ S.length b = 8 * l }):
-  s:S.seq UInt64.t { S.length s = l }
-=
+let rec seq_uint64_of_be l b =
   if S.length b = 0 then
     S.empty
   else
     let hd, tl = Seq.split b 8 in
     S.cons (uint64_of_be hd) (seq_uint64_of_be (l - 1) tl)
 
-let rec be_of_seq_uint64 (s: S.seq UInt64.t):
-  Tot (b:bytes { S.length b = 8 * S.length s })
-    (decreases (S.length s))
-=
+let rec be_of_seq_uint64 s =
   if S.length s = 0 then
     S.empty
   else
@@ -326,17 +214,7 @@ let rec be_of_seq_uint64 (s: S.seq UInt64.t):
 
 #set-options "--max_fuel 1 --max_ifuel 0 --z3rlimit 50"
 
-let rec offset_uint32_be (b: bytes) (n: nat) (i: nat):
-  Lemma
-    (requires (
-      S.length b = 4 * n /\
-      i < n))
-    (ensures (
-      S.index (seq_uint32_of_be n b) i == uint32_of_be (S.slice b (4 * i) (4 * i + 4))))
-    (decreases (
-      S.length b))
-    [ SMTPat (S.index (seq_uint32_of_be n b) i) ]
-=
+let rec offset_uint32_be (b: bytes) (n: nat) (i: nat) =
   if S.length b = 0 then
     false_elim ()
   else
@@ -346,17 +224,7 @@ let rec offset_uint32_be (b: bytes) (n: nat) (i: nat):
     else
       offset_uint32_be tl (n - 1) (i - 1)
 
-let rec offset_uint32_le (b: bytes) (n: nat) (i: nat):
-  Lemma
-    (requires (
-      S.length b = 4 * n /\
-      i < n))
-    (ensures (
-      S.index (seq_uint32_of_le n b) i == uint32_of_le (S.slice b (4 * i) (4 * i + 4))))
-    (decreases (
-      S.length b))
-    [ SMTPat (S.index (seq_uint32_of_le n b) i) ]
-=
+let rec offset_uint32_le (b: bytes) (n: nat) (i: nat) =
   if S.length b = 0 then
     false_elim ()
   else
@@ -366,17 +234,7 @@ let rec offset_uint32_le (b: bytes) (n: nat) (i: nat):
     else
       offset_uint32_le tl (n - 1) (i - 1)
 
-let rec offset_uint64_be (b: bytes) (n: nat) (i: nat):
-  Lemma
-    (requires (
-      S.length b = 8 * n /\
-      i < n))
-    (ensures (
-      S.index (seq_uint64_of_be n b) i == uint64_of_be (S.slice b (8 * i) (8 * i + 8))))
-    (decreases (
-      S.length b))
-    [ SMTPat (S.index (seq_uint64_of_be n b) i) ]
-=
+let rec offset_uint64_be (b: bytes) (n: nat) (i: nat) =
   if S.length b = 0 then
     false_elim ()
   else
@@ -386,17 +244,7 @@ let rec offset_uint64_be (b: bytes) (n: nat) (i: nat):
     else
       offset_uint64_be tl (n - 1) (i - 1)
 
-let rec offset_uint64_le (b: bytes) (n: nat) (i: nat):
-  Lemma
-    (requires (
-      S.length b = 8 * n /\
-      i < n))
-    (ensures (
-      S.index (seq_uint64_of_le n b) i == uint64_of_le (S.slice b (8 * i) (8 * i + 8))))
-    (decreases (
-      S.length b))
-    [ SMTPat (S.index (seq_uint64_of_le n b) i) ]
-=
+let rec offset_uint64_le (b: bytes) (n: nat) (i: nat) =
   if S.length b = 0 then
     false_elim ()
   else
@@ -419,14 +267,7 @@ let tail_cons (#a: Type) (hd: a) (tl: S.seq a): Lemma
 =
   ()
 
-let rec be_of_seq_uint32_append (s1 s2: S.seq U32.t): Lemma
-  (ensures (
-    S.equal (be_of_seq_uint32 (S.append s1 s2))
-      (S.append (be_of_seq_uint32 s1) (be_of_seq_uint32 s2))))
-  (decreases (
-    S.length s1))
-  [ SMTPat (S.append (be_of_seq_uint32 s1) (be_of_seq_uint32 s2)) ]
-=
+let rec be_of_seq_uint32_append s1 s2 =
   Classical.forall_intro_2 (tail_cons #U32.t); // TODO: this is a local pattern, remove once tail_cons lands in FStar.Seq.Properties
   if S.length s1 = 0 then begin
     assert (S.equal (be_of_seq_uint32 s1) S.empty);
@@ -449,14 +290,7 @@ let be_of_seq_uint32_base (s1: S.seq U32.t) (s2: S.seq U8.t): Lemma
 =
   ()
 
-let rec le_of_seq_uint32_append (s1 s2: S.seq U32.t): Lemma
-  (ensures (
-    S.equal (le_of_seq_uint32 (S.append s1 s2))
-      (S.append (le_of_seq_uint32 s1) (le_of_seq_uint32 s2))))
-  (decreases (
-    S.length s1))
-  [ SMTPat (S.append (le_of_seq_uint32 s1) (le_of_seq_uint32 s2)) ]
-=
+let rec le_of_seq_uint32_append s1 s2 =
   Classical.forall_intro_2 (tail_cons #U32.t); // TODO: this is a local pattern, remove once tail_cons lands in FStar.Seq.Properties
   if S.length s1 = 0 then begin
     assert (S.equal (le_of_seq_uint32 s1) S.empty);
@@ -479,14 +313,7 @@ let le_of_seq_uint32_base (s1: S.seq U32.t) (s2: S.seq U8.t): Lemma
 =
   ()
 
-let rec be_of_seq_uint64_append (s1 s2: S.seq U64.t): Lemma
-  (ensures (
-    S.equal (be_of_seq_uint64 (S.append s1 s2))
-      (S.append (be_of_seq_uint64 s1) (be_of_seq_uint64 s2))))
-  (decreases (
-    S.length s1))
-  [ SMTPat (S.append (be_of_seq_uint64 s1) (be_of_seq_uint64 s2)) ]
-=
+let rec be_of_seq_uint64_append s1 s2 =
   Classical.forall_intro_2 (tail_cons #U64.t); // TODO: this is a local pattern, remove once tail_cons lands in FStar.Seq.Properties
   if S.length s1 = 0 then begin
     assert (S.equal (be_of_seq_uint64 s1) S.empty);
@@ -509,12 +336,8 @@ let be_of_seq_uint64_base (s1: S.seq U64.t) (s2: S.seq U8.t): Lemma
 =
   ()
 
-let rec seq_uint32_of_be_be_of_seq_uint32 (n: nat) (s: S.seq U32.t) : Lemma
-  (requires (n == S.length s))
-  (ensures (seq_uint32_of_be n (be_of_seq_uint32 s) `S.equal` s))
-  (decreases n)
-  [SMTPat (seq_uint32_of_be n (be_of_seq_uint32 s))]
-= if n = 0
+let rec seq_uint32_of_be_be_of_seq_uint32 n s =
+  if n = 0
   then ()
   else begin
     assert (s `S.equal` S.cons (S.head s) (S.tail s));
@@ -524,12 +347,8 @@ let rec seq_uint32_of_be_be_of_seq_uint32 (n: nat) (s: S.seq U32.t) : Lemma
     S.lemma_append_inj (S.slice s' 0 4) (S.slice s' 4 (S.length s')) (be_of_uint32 (S.head s)) (be_of_seq_uint32 (S.tail s))
   end
 
-let rec be_of_seq_uint32_seq_uint32_of_be (n: nat) (s: S.seq U8.t) : Lemma
-  (requires (4 * n == S.length s))
-  (ensures (be_of_seq_uint32 (seq_uint32_of_be n s) `S.equal` s))
-  (decreases n)
-  [SMTPat (be_of_seq_uint32 (seq_uint32_of_be n s))]
-= if n = 0
+let rec be_of_seq_uint32_seq_uint32_of_be n s =
+  if n = 0
   then ()
   else begin
     S.lemma_split s 4;
@@ -545,12 +364,7 @@ let rec be_of_seq_uint32_seq_uint32_of_be (n: nat) (s: S.seq U8.t) : Lemma
     n_to_be_be_to_n 4 hd
   end
 
-let slice_seq_uint32_of_be (n: nat) (s: S.seq U8.t) (lo: nat) (hi: nat) : Lemma
-  (requires (4 * n == S.length s /\ lo <= hi /\ hi <= n))
-  (ensures (S.slice (seq_uint32_of_be n s) lo hi) `S.equal` seq_uint32_of_be (hi - lo) (S.slice s (4 * lo) (4 * hi)))
-= ()
+let slice_seq_uint32_of_be n s lo hi = ()
 
-let be_of_seq_uint32_slice (s: S.seq U32.t) (lo: nat) (hi: nat) : Lemma
-  (requires (lo <= hi /\ hi <= S.length s))
-  (ensures (be_of_seq_uint32 (S.slice s lo hi) `S.equal` S.slice (be_of_seq_uint32 s) (4 * lo) (4 * hi)))
-= slice_seq_uint32_of_be (S.length s) (be_of_seq_uint32 s) lo hi
+let be_of_seq_uint32_slice s lo hi =
+  slice_seq_uint32_of_be (S.length s) (be_of_seq_uint32 s) lo hi
